feat(proj1): first exercise almost completed

proj1/src/Ex1.dfy
@@ -23,15 +23,35 @@ function Serialize(a : aexpr) : seq<code>
   }
 }
 
+method Main() {
+    var result := Deserialize(Serialize(BinOp(Minus, BinOp(Plus, Val(1), Val(2)), BinOp(Minus, Val(1), Val(3)))));
+    print result;
+}
 
 /*
   Ex1.1
 */
 function Deserialize(cs : seq<code>) : seq<aexpr> 
 {
-  
+  if cs == [] then [] else DeserializeRec(cs, [])  
 }
 
+function DeserializeRec(cs: seq<code>, exprs: seq<aexpr>): seq<aexpr>
+{
+  if cs == []
+  then exprs
+  else DeserializeRec(cs[1..], DeserializeSingle(cs[0], exprs))
+}
+
+function DeserializeSingle(c: code, exprs: seq<aexpr>): seq<aexpr>
+{
+  match c {
+    case VarCode(s) => [Var(s)] + exprs
+    case ValCode(i) => [Val(i)] + exprs
+    case UnOpCode(uop) => if |exprs| < 1 then [] else [UnOp(uop, exprs[0])] + exprs[1..]
+    case BinOpCode(bop) => if |exprs| < 2 then [] else [BinOp(bop, exprs[0], exprs[1])] + exprs[2..]
+  }
+}
 
 /*
   Ex1.2
@@ -39,7 +59,68 @@ function Deserialize(cs : seq<code>) : seq<aexpr>
 lemma DeserializeProperty(e : aexpr)
   ensures Deserialize(Serialize(e)) == [ e ]
 {
- 
+  match e {
+    // I was expecting the base cases to require 0 stuff
+    case Var(s) => {
+        // Does this need to be in calculational style ?
+        assert(Deserialize(Serialize(e)) == DeserializeRec([VarCode(s)], []));
+    }
+    case Val(i) => {
+        // Does this need to be in calculational style ?
+        assert(Deserialize(Serialize(e)) == DeserializeRec([ValCode(i)], []));
+    }
+    case UnOp(op, a1) => calc {
+          Deserialize(Serialize(e));
+        ==  { assert Serialize(e) == Serialize(e) + []; }
+          Deserialize(Serialize(e) + []);
+        == { DeserializeSegments(UnOp(op,a1), [], []); }
+          [UnOp(op, a1)];
+    }
+    case BinOp(op, a1, a2) => calc {
+          Deserialize(Serialize(e));
+        ==  { assert Serialize(e) == Serialize(e) + []; }
+          Deserialize(Serialize(e) + []);
+        == { DeserializeSegments(BinOp(op,a1,a2), [], []); }
+          [BinOp(op, a1, a2)];
+    }
+  }
+}
+
+lemma DeserializeSegments(a: aexpr, ops: seq<code>, l: seq<aexpr>)
+  ensures DeserializeRec(Serialize(a) + ops, l) == DeserializeRec(ops, [a] + l)
+{
+  match a {
+    case Var(s) => {}
+    case Val(i) => {}
+    case UnOp(op, a1) => calc {
+        DeserializeRec(Serialize(UnOp(op, a1)) + ops, l);
+      ==
+        DeserializeRec(Serialize(a1) + [UnOpCode(op)] + ops, l);
+      == {assert Serialize(a1) + [UnOpCode(op)] + ops == Serialize(a1) + ([UnOpCode(op)] + ops); }
+        DeserializeRec(Serialize(a1) + ([UnOpCode(op)] + ops), l);
+      == { DeserializeSegments(a1, [UnOpCode(op)] + ops, l); }
+        DeserializeRec([UnOpCode(op)] + ops, [a1] + l);
+      ==
+        DeserializeRec(ops, [a] + l);
+    }
+    case BinOp(op, a1, a2) => calc {
+        DeserializeRec(Serialize(BinOp(op, a1, a2)) + ops, l);
+      ==
+        DeserializeRec(Serialize(a2) + Serialize(a1) + [ BinOpCode(op) ] + ops, l);
+      == {assert Serialize(a2) + Serialize(a1) + [ BinOpCode(op) ] + ops == Serialize(a2) + (Serialize(a1) + [ BinOpCode(op) ] + ops); }
+        DeserializeRec(Serialize(a2) + (Serialize(a1) + [ BinOpCode(op) ] + ops), l);
+      ==
+        DeserializeRec(Serialize(a1) + [ BinOpCode(op) ] + ops, [a2] + l);
+      == {assert Serialize(a1) + [ BinOpCode(op) ] + ops == Serialize(a1) + ([ BinOpCode(op) ] + ops); }
+        DeserializeRec(Serialize(a1) + ([ BinOpCode(op) ] + ops), [a2] + l);
+      == { DeserializeSegments(a1, [ BinOpCode(op) ] + ops, [a2] + l); }
+        DeserializeRec([ BinOpCode(op) ] + ops, [a1] + ([a2] + l));
+      == {assert [a1, a2] + l == [a1] + ([a2] + l); }
+        DeserializeRec([ BinOpCode(op) ] + ops, [a1, a2] + l);
+      ==
+        DeserializeRec(ops, [BinOp(op, a1, a2)] + l);
+    }
+  }
 }
 
 
@@ -48,38 +129,165 @@ lemma DeserializeProperty(e : aexpr)
 */
 function SerializeCodes(cs : seq<code>) : seq<nat> 
 {
+  if cs == [] then [] else SerializeSingleCode(cs[0]) + SerializeCodes(cs[1..])
+}
 
+function SerializeSingleCode(cs : code) : seq<nat> 
+{
+  match cs {
+    case VarCode(s) => [0, |s|] + s
+    case ValCode(i) => [1, i]
+    case UnOpCode(uop) => [2]
+    case BinOpCode(bop) => match bop {
+      case Plus => [3, 0]
+      case Minus => [3, 1]
+    }
+  }
 }
 
 function DeserializeCodes(ints : seq<nat>) : seq<code> {
-  
+  DeserializeCodesRec(ints, []) 
 }
 
+function DeserializeCodesRec(ints : seq<nat>, cs: seq<code>) : seq<code>
 
-/*
-  Ex1.4
-*/
+{
+  if ints == []
+  then cs
+  else match ints[0] {
+    case 0 => 
+      if |ints| < 2 then []
+      else if |ints[2..]| < ints[1] then []
+      else DeserializeCodesRec(ints[2..][(ints[1])..], [VarCode(ints[2..][..(ints[1])])] + cs)
+    case 1 =>
+      if |ints| < 2 then []
+      else DeserializeCodesRec(ints[2..], [ValCode(ints[1])] + cs)
+    case 2 => DeserializeCodesRec(ints[1..], [UnOpCode(Neg)] + cs)
+    case 3 => if |ints| < 2
+      then []
+      else match ints[1] {
+        case 0 => DeserializeCodesRec(ints[2..], [BinOpCode(Plus)] + cs)
+        case 1 => DeserializeCodesRec(ints[2..], [BinOpCode(Minus)] + cs)
+        case _ => []
+      }
+    case _ => [] // invalid serialization
+  }
+}
+
+// /*
+//   Ex1.4
+// */
 lemma DeserializeCodesProperty(cs : seq<code>)
   ensures DeserializeCodes(SerializeCodes(cs)) == cs
 {
+  if cs == [] { }
+  else {
+    calc {
+        DeserializeCodes(SerializeCodes(cs));
+      ==
+        DeserializeCodes(SerializeSingleCode(cs[0]) + SerializeCodes(cs[1..]));
+      ==
+        DeserializeCodesRec(SerializeSingleCode(cs[0]) + SerializeCodes(cs[1..]), []);
+      == 
+        DeserializeCodes(SerializeSingleCode(cs[0])) + DeserializeCodes(SerializeCodes(cs[1..]));
+      == { DeserializeSingleCodeProperty(cs[0]); }
+        [cs[0]] + DeserializeCodes(SerializeCodes(cs[1..]));
+      ==
+        [cs[0]] + cs[1..];
+      ==
+        cs;
+    }
+  }
 }
 
-/*
-  Ex1.5
-*/
+lemma DeserializeSingleCodeProperty(c : code)
+  ensures DeserializeCodes(SerializeSingleCode(c)) == [c]
+{
+  match c {
+    case VarCode(s) => {
+      var ints := [0, |s|] + s;
+      calc {
+          DeserializeCodes(SerializeSingleCode(VarCode(s)));
+        ==
+          DeserializeCodesRec([0, |s|] + s, []);
+        == 
+          DeserializeCodesRec(ints, []);
+        ==
+          DeserializeCodesRec(ints[2..][(ints[1])..], [VarCode(ints[2..][..(ints[1])])] + []);
+        ==
+          DeserializeCodesRec([], [VarCode(ints[2..][..(ints[1])])] + []);
+        ==
+          DeserializeCodesRec([], [VarCode(s[..(ints[1])])] + []);
+        ==
+          DeserializeCodesRec([], [VarCode(s[..(|s|)])] + []);
+        == { assert s[..|s|] == s; }
+          DeserializeCodesRec([], [VarCode(s)] + []);
+        ==
+          [c];
+      }
+    }
+    case ValCode(i) => calc {
+          DeserializeCodes(SerializeSingleCode(ValCode(i)));
+        ==
+          DeserializeCodes([1, i]);
+        ==
+          DeserializeCodes([1, i]);
+        ==
+          DeserializeCodesRec([], [ValCode(i)] + []);
+        ==
+          [c];
+    }
+    case UnOpCode(uop) => calc {
+          DeserializeCodes(SerializeSingleCode(UnOpCode(uop)));
+        ==
+          DeserializeCodesRec([], [UnOpCode(Neg)] + []);
+        == {assert uop == Neg;}
+          [c];
+    }
+    // Can i use the match inside a calc ?
+    case BinOpCode(bop) => match bop {
+      case Plus => calc {
+          DeserializeCodes(SerializeSingleCode(BinOpCode(bop)));
+        == { assert Plus == bop; } // why is this needed?
+          DeserializeCodesRec([], [BinOpCode(Plus)] + []);
+        ==
+          [c];
+      }
+      case Minus => calc {
+          DeserializeCodes(SerializeSingleCode(BinOpCode(bop)));
+        ==
+          DeserializeCodesRec([], [BinOpCode(Minus)] + []);
+        ==
+          [c];
+      }
+    }
+  }
+}
+
+// /*
+//   Ex1.5
+// */
 function FullSerialize(e : aexpr) : seq<nat> {
- 
+  SerializeCodes(Serialize(e))
 }
 
 function FullDeserealize(nats : seq<nat>) : seq<aexpr> {
- 
+  Deserialize(DeserializeCodes(nats))
 }
 
-/*
-  Ex1.6
-*/
+// /*
+//   Ex1.6
+// */
 lemma FullDeserealizeProperty(e : aexpr)
   ensures FullDeserealize(FullSerialize(e)) == [ e ]
 {
-    
+  calc {
+      FullDeserealize(FullSerialize(e));
+    ==
+      Deserialize(DeserializeCodes(SerializeCodes(Serialize(e))));
+    == { DeserializeCodesProperty(Serialize(e)); }
+      Deserialize((Serialize(e)));
+    == { DeserializeProperty(e); }
+      [ e ];
+  }
 }
